add syntax for statements and evaluation rules

proof-of-soundness/c-subset-syntax.v
@@ -1,8 +1,15 @@
 Require Import Coq.Strings.String.
 Require Import Coq.Lists.List.
 Require Import ZArith.
-Open Scope Z_scope.
+Require Import Coq.FSets.FMapList.
+Require Import Coq.Strings.String.
 
+Open Scope Z_scope.
+Open Scope string_scope.
+
+
+(* I'm not sure if this is correct, but it seems to work *)
+Definition state : Set := list (string * Z).
 
 
 Inductive unop : Type :=
@@ -15,39 +22,42 @@ Inductive binop : Type :=
   | Mul
   | Div.
 
-Inductive const_exp : Type :=
+Inductive const_expr : Type :=
   | ConstNum (z : Z)
-  | ConstParenExpr (ce : const_exp)
-  | ConstUnOp (uo : unop) (ce : const_exp)
-  | ConstBinOp (ce1 ce2 : const_exp) (bo : binop).
+  | ConstParenExpr (ce : const_expr)
+  | ConstUnExpr (uo : unop) (ce : const_expr)
+  | ConstBinExpr (ce1 ce2 : const_expr) (bo : binop).
 
-Inductive var_exp : Type :=
+Inductive var_expr : Type :=
   | X (x : string)
   | Num (z : Z)
-  | ParenExpr (va : var_exp)
-  | UnOp (uo : unop) (va : var_exp)
-  | BinOp (va1 va2 : var_exp) (bo : binop)
-  | Assign (va1 va2 : var_exp)
-  | CallOrInvoke (x : string) (vas: list var_exp).
+  | ParenExpr (va : var_expr)
+  | UnExpr (uo : unop) (va : var_expr)
+  | BinExpr (va1 va2 : var_expr) (bo : binop)
+  | Assign (va1 va2 : var_expr)
+  | CallOrInvoke (x : string) (vas: list var_expr).
 
-Inductive exp : Type :=
-  | ConstExpr (ce : const_exp)
-  | VarExpr (va : var_exp).
+Inductive expr : Type :=
+  | ConstExpr (ce : const_expr)
+  | VarExpr (va : var_expr).
 
 (* TODO: Make this meaningful*)
 Definition lookup (x:string) : Z := 1.
 
-Fixpoint ceval (ce : const_exp) : Z :=
+(* TODO: Add state to these evaluation rules.
+   May have to define evaluation as a relation instead of as
+   a function *)
+Fixpoint ceval (ce : const_expr) : Z :=
   match ce with
   | ConstNum z => z
   | ConstParenExpr ce => ceval ce
-  | ConstUnOp uo ce =>
+  | ConstUnExpr uo ce =>
     let v := ceval ce in
       match uo with
      | Positive => id v
      | Negative => - v
      end
-  | ConstBinOp ce1 ce2 bo =>
+  | ConstBinExpr ce1 ce2 bo =>
     let v1 := (ceval ce1) in
     let v2 := (ceval ce2) in
       match bo with
@@ -59,18 +69,18 @@ Fixpoint ceval (ce : const_exp) : Z :=
 end.
 
 
-Fixpoint veval (va : var_exp) : Z :=
+Fixpoint veval (va : var_expr) : Z :=
   match va with
   | X x => lookup x
   | Num n => n
   | ParenExpr va => veval va
-  | UnOp uo va =>
+  | UnExpr uo va =>
     let v := veval va in
       match uo with
       | Positive => id v
       | Negative => - v
       end
-  | BinOp va1 va2 bo =>
+  | BinExpr va1 va2 bo =>
     let v1 := veval va1 in
     let v2 := veval va2 in
       match bo with
@@ -88,7 +98,7 @@ Fixpoint veval (va : var_exp) : Z :=
   end.
 
 
-Definition eeval (e : exp) : Z :=
+Definition eeval (e : expr) : Z :=
   match e with
   | ConstExpr ce => ceval ce
   | VarExpr va => veval va
@@ -96,22 +106,79 @@ Definition eeval (e : exp) : Z :=
 
 Lemma nnzeq : forall z : Z,
   - - z = z.
+Proof. induction z as []; reflexivity. Qed.
+
+(* Proof that negation is involute in our language; i.e.,
+that applying the unary operation negate to a constant exprression twice
+results in the same value.*)
+Theorem neg_neg_equal_ce : forall ce : const_expr,
+  ceval (ConstUnExpr Negative (ConstUnExpr Negative ce)) = ceval ce.
 Proof.
-induction z as [].
-- (* 0 *)     simpl. reflexivity.
-- (* z > 0 *) simpl. reflexivity.
-- (* z < 0 *) simpl. reflexivity.
+  induction ce as []; simpl; rewrite nnzeq; reflexivity.
 Qed.
 
-(* Proof that the negation is involute in our language; i.e.,
-that applying the unary operation negate to a constant expression twice
-results in the same value.*)
-Theorem neg_neg_equal_ce : forall ce : const_exp,
-ceval (ConstUnOp Negative (ConstUnOp Negative ce)) = ceval ce.
+(* Proof that adding zero any constant exprression results in the same
+value *)
+Theorem optimize_ce: forall ce : const_expr,
+  ceval (ConstBinExpr (ConstNum 0) ce Plus) = ceval ce.
 Proof.
-  induction ce as [].
-  - (* ConstNum *)        simpl. rewrite nnzeq. reflexivity.
-  - (* ConstParentExpr *) simpl. rewrite nnzeq. reflexivity.
-  - (* ConstUnOp *)       simpl. rewrite nnzeq. reflexivity.
-  - (* ConstBinOp *)      simpl. rewrite nnzeq. reflexivity.
+  induction ce as []; reflexivity.
 Qed.
+
+
+(* Define evaluation as a relation instead of a function *)
+Inductive cevalR : const_expr -> Z -> Prop :=
+  | E_ConstNum (z : Z) : cevalR (ConstNum z) z.
+
+
+Inductive stmt : Type :=
+  (* We may not need this, I added it to make the evaluation rule
+     for compound statements easier to define *)
+  | Skip
+  | ExprStmt (e : expr)
+  (* TODO: Add compound statemetns *)
+  (* TODO: Allow for ifs without else branches *)
+  | IfElseStmt (cond: expr) (s0 s1: stmt)
+  | WhileStmt (cond : expr) (s0 : stmt).
+
+
+Reserved Notation
+  "st '=[' s ']=>' st'"
+  (at level 90, left associativity).
+(* Define the evaluation rule for statements as a
+   relation instead of an inductive type to permite the non-
+   determinism introduced by while loops *)
+Inductive stmtevalR : stmt -> state -> state -> Prop :=
+  (* A skip statement does not change the state *)
+  | E_Skip : forall st,
+    st =[ Skip ]=> st
+  (* An expr statement does not change the state (for now) *)
+  | E_ExprStmt : forall st e,
+    st =[ ExprStmt e ]=> st
+  (* An if statement whose expression evaluates to
+     has their else statement evaluated *)
+  | E_IfElseFalse : forall st st' e s0 s1,
+    eeval e = 0 ->
+    st =[ s1 ]=> st' ->
+    st =[ IfElseStmt e s0 s1 ]=> st'
+  (* An if statement whose expression evaluates a nonzero value
+     has their true statement evaluated *)
+  | E_IfElseTrue : forall st st' e s0 s1,
+    eeval e <> 0 ->
+    st =[ s0 ]=> st' ->
+    st =[ IfElseStmt e s0 s1 ]=> st'
+  (* A while statement whose expression evaluates to 0
+     does not change the state *)
+  | E_WhileFalse : forall st e s0,
+    eeval e = 0 ->
+    st =[ WhileStmt e s0 ]=> st
+  (* This is the interesting one.
+     A while statement whose expression evaluates to a nonzero value
+     has their body evaluated, then they themselves are evaluated
+     again with the updated state *)
+  | E_WhileTrue : forall st st' st'' e s0,
+    eeval e <> 0 ->
+    st =[ s0 ]=> st' ->
+    st' =[ WhileStmt e s0 ]=> st'' ->
+    st =[ WhileStmt e s0 ]=> st''
+  where "st '=[' s ']=>' st'" := (stmtevalR s st st') : type_scope.
